11: Replaced the old code

Bellman.dfy
@@ -1,33 +1,118 @@
-datatype Node = Node(id: int, neighbors: set<Node>)
+datatype Weight = W(val: int)
+datatype Node = V(id: int)
 
-class Graph
-  {
-  var nodes: set<Node>
+datatype Edge = Edge(source: Node, destination: Node, weight: Weight)
+datatype Graph = Graph(nodes: set<Node>, edges: set<Edge>)
 
-  constructor(nodes: set<Node>)
+function edge_weight(e: Edge): int
+{
+  match e
+  case Edge(from_where, to_where, W(w)) => w
+}
+
+function from_where(e: Edge): Node
+{
+  match e
+  case Edge(from_where, to_where, W(w)) => from_where
+}
+
+function to_where(e: Edge): Node
+{
+  match e
+  case Edge(from_where, to_where, W(w)) => to_where
+}
+
+function nodes_in_graph(g: Graph): set<Node>
+{
+  match g
+  case Graph(v, e) => v
+}
+
+function edges_in_graph(g: Graph): set<Edge>
+{
+  match g
+  case Graph(v, e) => e
+}
+
+predicate isValid(graph: Graph)
+{
+  forall e :: e in graph.edges ==> e.source in graph.nodes && e.destination in graph.nodes
+}
+
+method Main(){
+  var node1 := V(1);
+  var node2 := V(2);
+  var node3 := V(3);
+
+  var edge1 := Edge(node1, node2, W(2));
+  var edge2 := Edge(node2,node3, W(4));
+
+  var graph1 := Graph({node1,node2,node3}, {edge1,edge2});
+}
+
+predicate EmptySet<T(==)>() { {} is set<T> }
+
+method check_if_set_empty(s: set<int>) returns (IsEmpty:bool)
+{
+  IsEmpty := s == {};
+}
+
+datatype MyInt = Valid(n: int) | MinValue
+
+method testMinValue(x: MyInt) returns (isMin: bool)
+{
+  isMin := match x {
+    case MinValue => true
+    case Valid(_) => false
+  };
+}
+
+/*
+method RelaxEdges(distance: array<MyInt>, predecessor: array<int>)
+  returns (success: bool)
+  requires distance.Length == vertices
+  requires predecessor.Length == vertices
+  modifies distance, predecessor
+  ensures success ==> forall u, v, w :: (u, v, w) in edges ==> distance[v] <= distance[u] + w
+{
+  success := true;
+
+  var i: nat := 0;
+
+  while i < vertices - 1
+    invariant 0 <= i <= vertices - 1
+    invariant forall u, v, w :: (u, v, w) in edges && distance[u] != MyInt.MinValue ==> distance[v] <= distance[u] + w
   {
-    this.nodes := nodes;
+    for i := 0 to |edges|
+
+    {
+      var egde := edges[i];
+      var u, v, w := edge.0, edge.1, edge.2;
+
+      if distance[u] != MyInt.MinValue && distance[u] + w < distance[v] {
+        distance[v] := distance[u] + w;
+        predecessor[v] := u;
+      }
+    }
+    i := i + 1;
   }
+  success := forall u, v, w :: (u, v, w) in edges && distance[u] != MyInt.MinValue ==> distance[v] <= distance[u] + w;
 }
 
-function CreateNode(id: int): Node
+*/
+method hasNegativeCycle(graph: Graph) returns (hasNegative: bool)
 {
-  Node(id, {})
+  var nodess := graph.nodes;
+  var edgess := graph.edges;
+
+  if nodess == {} {
+    hasNegative := false;
+    return;
+  }
+  else{
+    hasNegative := true;
+    return;
+  }
+
 }
 
-function AddNeighbors(node: Node, neighbors: set<Node>): Node
-{
-  Node(node.id, neighbors)
-}
-
-method Main() {
-  var node1 := CreateNode(1);
-  var node2 := CreateNode(2);
-  var node3 := CreateNode(3);
-
-  var updatedNode1 := AddNeighbors(node1, {node2, node3});
-  var updatedNode2 := AddNeighbors(node2, {node1, node3});
-  var updatedNode3 := AddNeighbors(node3, {node1, node2});
-
-  var graph := new Graph({updatedNode1, updatedNode2, updatedNode3});
-}
